src/syntax/FStar.Syntax.Resugar.fsti
@@ -38,7 +38,7 @@ val resugar_sigelt: S.sigelt -> option A.decl
 val resugar_comp: S.comp -> A.term
 val resugar_pat: S.pat -> FlatSet.t S.bv -> A.pattern
 val resugar_universe: S.universe -> Range.range -> A.term
-val resugar_binder: S.binder -> Range.range -> option A.binder
+val resugar_binder: S.binder -> Range.range -> A.binder
 val resugar_tscheme: S.tscheme -> A.decl
 val resugar_eff_decl: eff_decl -> A.decl
 
@@ -47,6 +47,6 @@ val resugar_sigelt': DsEnv.env -> S.sigelt -> option A.decl
 val resugar_comp': DsEnv.env -> S.comp -> A.term
 val resugar_pat': DsEnv.env -> S.pat -> FlatSet.t S.bv -> A.pattern
 val resugar_universe': DsEnv.env -> S.universe -> Range.range -> A.term
-val resugar_binder': DsEnv.env -> S.binder -> Range.range -> option A.binder
+val resugar_binder': DsEnv.env -> S.binder -> Range.range -> A.binder
 val resugar_tscheme': DsEnv.env -> S.tscheme -> A.decl
 val resugar_eff_decl': DsEnv.env -> eff_decl -> A.decl
